Simple simulation

src/sequential/SequentialDef.v
@@ -16,7 +16,7 @@ Require Import Event.
 Set Implicit Arguments.
 
 Module Perm.
-  Variant t :=
+  Variant t: Type :=
   | none
   | full
   .
@@ -37,26 +37,64 @@ Variant flag :=
 
 Definition flag_le (f_src f_tgt: flag): bool :=
   match f_src, f_tgt with
-  | promised, _ => false
   | written, _ => true
   | unwritten, unwritten => true
+  | unwritten, promised => true
+  | promised, promised => true
   | _, _ => false
   end.
 
+Program Instance flag_le_PreOrder: PreOrder flag_le.
+Next Obligation.
+Proof.
+  ii. destruct x; ss.
+Qed.
+Next Obligation.
+Proof.
+  ii. destruct x, y, z; ss.
+Qed.
+
 Definition Perms := Loc.t -> Perm.t.
 
+Module SeqCell.
+   Definition t := (Const.t * flag)%type.
+
+   Definition le (c0 c1: t): Prop :=
+     match c0, c1 with
+     | (v0, f0), (v1, f1) => v0 = v1 /\ flag_le f0 f1
+     end.
+
+   Program Instance le_PreOrder: PreOrder le.
+   Next Obligation.
+   Proof.
+     ii. destruct x; ss. split; auto. refl.
+   Qed.
+   Next Obligation.
+   Proof.
+     ii. destruct x, y, z; ss.
+     des. subst. splits; auto. etrans; eauto.
+   Qed.
+End SeqCell.
+
+
 Module SeqMemory.
-  Definition t := Loc.t -> Const.t * flag.
+  Definition t := Loc.t -> SeqCell.t.
 
   Definition update (loc: Loc.t) (val: Const.t) (m: t): t :=
     fun loc' => if Loc.eq_dec loc' loc then (val, written) else (m loc').
 
   Definition le (m_src m_tgt: t): Prop :=
-    forall loc,
-      match (m_src loc), (m_tgt loc) with
-      | (v_src, f_src), (v_tgt, f_tgt) =>
-        v_src = v_tgt /\ flag_le f_src f_tgt
-      end.
+    forall loc, SeqCell.le (m_src loc) (m_tgt loc).
+
+  Program Instance le_PreOrder: PreOrder le.
+  Next Obligation.
+  Proof.
+    ii. refl.
+  Qed.
+  Next Obligation.
+  Proof.
+    ii. etrans; eauto.
+  Qed.
 End SeqMemory.
 
 
@@ -130,177 +168,171 @@ Section LANG.
     :
       na_step p e (mk st0 m0) (mk st1 m1)
   .
+
+  Variant na_opt_step (p: Perms): MachineEvent.t -> t -> t -> Prop :=
+  | na_opt_step_some
+      e st0 st1
+      (STEP: na_step p e st0 st1)
+    :
+      na_opt_step p e st0 st1
+  | na_opt_step_none
+      st0
+    :
+      na_opt_step p MachineEvent.silent st0 st0
+  .
 End LANG.
 End SeqState.
 
 
-Variant sort :=
-| rlx (* no change *)
-| srlx (
-| acq
-| rel
-| relacq
-| event
-| upd
-.
-
-  perms
-  mem_src
-  mem_tgt
-  written_src
-  written_tgt
-  proms_src
-
-
-Variant at_step:
-  forall
-    (s: sort)
-    (p0: Perms)
-    (m_src0: SeqMemory.t)
-    (m_tgt0: SeqMemory.t)
-    (proms0: Proms)
-    (p1: Perms)
-    (m_src1: SeqMemory.t)
-    (m_tgt1: SeqMemory.t)
-    (proms1: Proms), Prop :=
-| at_step_rlx
-    p m_src m_tgt proms
-  :
-    at_step
-      rlx
-      p m_src m_tgt proms
-      p m_src m_tgt proms
-| at_step
-
-(* srlx *)
-| (* rel *)
-| (* acq *)
-
-
-| at_step_srlx
-    p m_src m_tgt proms
-  :
-    at_step
-      rlx
-      p m_src m_tgt proms
-      p m_src m_tgt proms
-.
-
-
-
-
-
-Variant at_step:
-  forall
-    (p0: Perms)
-    (m_src0: SeqMemory.t)
-    (m_tgt0: SeqMemory.t)
-    (proms0: Proms)
-    (p1: Perms)
-    (m_src1: SeqMemory.t)
-    (m_tgt1: SeqMemory.t)
-    (proms1: Proms), Prop :=
-| at_step_rlx
-
-
-
-    rlx fence
-    rlx
-
-
-    rlx/plain load
-    rlx/plain store
-    srlx store
-    acq load
-    rel store
-    upd
-
-
-
-
-
-Module Released.
-  Definition t := Loc.t -> option (Const.t * flag).
-
-  Definition le (rels0 rels: t): Prop :=
-    forall loc,
-      match (rels0 loc), (rels1 loc) with
-      | Some (
-
-
-
-Definition released_vals: Type := Loc.t -> option (Comn
-
-Definition mem_diff:
-
-
 Variant diff :=
-| diff_rlx
-| diff_rel (* (val: Const.t) (f: flag) *)
-| diff_acq (val: Const.t)
-| diff_relacq (* (valw: Const.t) (f: flag) *) (valr: Const.t)
+| diff_rlx (* no change *)
+| diff_acq
+| diff_rel
+| diff_reset
 .
 
 Definition diffs := Loc.t -> diff.
 
-Definition is_acq (d: diff): bool :=
-  match d with
-  | diff_acq _  => true
-  | _ => false
+Definition update_mem
+           (d: diffs) (v_diff: Loc.t -> Const.t) (m0: SeqMemory.t): SeqMemory.t :=
+  fun loc =>
+    match (d loc) with
+    | diff_rlx | diff_rel => m0 loc
+    | diff_acq | diff_reset => (v_diff loc, unwritten)
+    end.
+
+Definition update_perm (d: diffs) (p0: Perms): Perms :=
+  fun loc =>
+    match (d loc) with
+    | diff_rlx | diff_reset => p0 loc
+    | diff_acq => Perm.full
+    | diff_rel => Perm.none
+    end.
+
+Definition match_mem (d: diffs) (mem_src mem_tgt: SeqMemory.t) :=
+  forall loc,
+    match (d loc) with
+    | diff_rel | diff_reset => SeqCell.le (mem_src loc) (mem_tgt loc)
+    | _ => True
+    end.
+
+
+Definition wf_diff_perms (d: diffs) (p: Perms): Prop :=
+  forall loc,
+    match (d loc), (p loc) with
+    | diff_rlx, _ => True
+    | diff_rel, Perm.full => True
+    | diff_reset, Perm.full => True
+    | diff_acq, Perm.none => True
+    | _, _ => False
+    end.
+
+Definition wf_diff_event (d: diffs) (e: ProgramEvent.t): Prop :=
+  match e with
+  | ProgramEvent.syscall _ => True
+  | ProgramEvent.read loc _ ord =>
+    forall loc' (NEQ: loc' <> loc),
+      match (d loc') with
+      | diff_rel | diff_reset => False
+      | diff_acq => Ordering.le Ordering.acqrel ord
+      | diff_rlx => True
+      end
+  | ProgramEvent.write loc _ ord =>
+    forall loc' (NEQ: loc' <> loc),
+      match (d loc') with
+      | diff_acq | diff_reset => False
+      | diff_rel => Ordering.le Ordering.acqrel ord
+      | diff_rlx => True
+      end
+  | ProgramEvent.update loc _ _ ordr ordw =>
+    forall loc' (NEQ: loc' <> loc),
+      match (d loc') with
+      | diff_reset => False
+      | diff_rel => Ordering.le Ordering.acqrel ordw
+      | diff_acq => Ordering.le Ordering.acqrel ordr
+      | diff_rlx => True
+      end
+  | ProgramEvent.fence ordr ordw =>
+    forall loc',
+      match (d loc') with
+      | diff_reset => False
+      | diff_rel => Ordering.le Ordering.acqrel ordw
+      | diff_acq => Ordering.le Ordering.acqrel ordr
+      | diff_rlx => True
+      end
+  | _ => True
   end.
 
-Definition is_rel (d: diff): bool :=
-  match d with
-  | diff_rel => true
-  | _ => false
+Definition is_atomic_event (e: ProgramEvent.t): Prop :=
+  match e with
+  | ProgramEvent.silent | ProgramEvent.failure => False
+  | ProgramEvent.syscall _ | ProgramEvent.fence _ _ => True
+  | ProgramEvent.read _ _ ord => Ordering.le Ordering.plain ord
+  | ProgramEvent.write _ _ ord => Ordering.le Ordering.plain ord
+  | ProgramEvent.update _ _ _ ordr ordw =>
+    Ordering.le Ordering.plain ordr /\ Ordering.le Ordering.plain ordw
   end.
 
-Definition is_rlx (d: diff): bool :=
-  match d with
-  | diff_rlx => true
-  | _ => false
-  end.
 
-Variant wf_diff (d: diffs): forall (e: ProgramEvent.t), Prop :=
-| wf_diff_syscall
-    e
-  :
-    wf_diff d (ProgramEvent.syscall e)
-| wf_diff_fence
-    ordr ordw
-    (ACQ: forall loc (ORD: is_acq (d loc)), Ordering.le Ordering.acqrel ordr)
-    (REL: forall loc (ORD: is_rel (d loc)), Ordering.le Ordering.acqrel ordw)
-  :
-    wf_diff d (ProgramEvent.fence ordr ordw)
-| wf_diff_read
-    loc val ord
-    (REL: forall loc' (NEQ: loc' <> loc) (ORD: is_rel (d loc)), False)
-    (ACQ: forall loc' (NEQ: loc' <> loc) (ORD: is_acq (d loc)),
-        Ordering.le Ordering.acqrel ord)
-    (NA: Ordering.le Ordering.plain ord)
-  :
-    wf_diff d (ProgramEvent.read loc val ord)
-| wf_diff_write
-    loc val ord
-    (ACQ: forall loc' (NEQ: loc' <> loc) (ORD: is_acq (d loc)), False)
-    (REL: forall loc' (NEQ: loc' <> loc) (ORD: is_rel (d loc)),
-        Ordering.le Ordering.acqrel ord)
-    (NA: Ordering.le Ordering.plain ord)
-  :
-    wf_diff d (ProgramEvent.write loc val ord)
-| wf_diff_update
-    loc valr valw ordr ordw
-    (ACQ: forall loc' (NEQ: loc' <> loc) (ORD: is_acq (d loc)),
-        Ordering.le Ordering.acqrel ordr)
-    (REL: forall loc' (NEQ: loc' <> loc) (ORD: is_rel (d loc)),
-        Ordering.le Ordering.acqrel ordw)
-    (ORDR: Ordering.le Ordering.plain ordr)
-    (ORDW: Ordering.le Ordering.plain ordw)
-  :
-    wf_diff d (ProgramEvent.update loc valr valw ordr ordw)
-.
+Section SIMULATION.
+  Variable lang_src: language.
+  Variable lang_tgt: language.
 
-Variant update_perms (d: diffs) (p0 p1: perms)
+  Variable sim_terminal: forall (st_src:(Language.state lang_src)) (st_tgt:(Language.state lang_tgt)), Prop.
+
+  Definition _sim_seq
+             (sim_seq:
+                forall
+                  (p0: Perms)
+                  (st_src0: SeqState.t lang_src)
+                  (st_tgt0: SeqState.t lang_tgt), Prop)
+    :
+      forall
+        (p0: Perms)
+        (st_src0: SeqState.t lang_src)
+        (st_tgt0: SeqState.t lang_tgt), Prop :=
+    fun p0 st_src0 st_tgt0 =>
+      (<<TERMINAL:
+         forall (TERMINAL_TGT: lang_tgt.(Language.is_terminal) st_tgt0.(SeqState.state)),
+         exists st_src1,
+           (<<STEPS: rtc (SeqState.na_step p0 MachineEvent.silent) st_src0 st_src1>>) /\
+           (<<TERMINAL_SRC: lang_src.(Language.is_terminal) st_src1.(SeqState.state)>>) /\
+           (<<TERMINAL: sim_terminal st_src1.(SeqState.state) st_tgt0.(SeqState.state)>>)>>) /\
+      (<<NASTEP:
+         forall st_tgt1 e (STEP_TGT: SeqState.na_step p0 e st_tgt0 st_tgt1),
+         exists st_src1 st_src2,
+           (<<STEPS: rtc (SeqState.na_step p0 MachineEvent.silent) st_src0 st_src1>>) /\
+           (<<STEP: SeqState.na_opt_step p0 e st_src1 st_src2>>) /\
+           (<<SIM: sim_seq p0 st_src2 st_tgt1>>)>>) /\
+      (<<ATSTEP:
+         forall st_tgt1 e
+                (STEP_TGT: lang_tgt.(Language.step) e st_tgt0.(SeqState.state) st_tgt1)
+                (ATOMIC: is_atomic_event e),
+         exists st_src1 st_src2,
+           (<<STEPS: rtc (SeqState.na_step p0 MachineEvent.silent) st_src0 st_src1>>) /\
+           (<<STEP: lang_src.(Language.step) e st_src1.(SeqState.state) st_src2>>) /\
+           (<<SIM: forall d v_diff
+                          (DIFF: wf_diff_event d e)
+                          (PERM: wf_diff_perms d p0),
+               (<<MEM: match_mem d st_src1.(SeqState.memory) st_tgt0.(SeqState.memory)>>) /\
+               (<<SIM: sim_seq (update_perm d p0)
+                           (SeqState.mk _ st_src2 (update_mem d v_diff st_src1.(SeqState.memory)))
+                           (SeqState.mk _ st_tgt1 (update_mem d v_diff st_tgt0.(SeqState.memory)))>>)>>)>>).
+
+  Lemma sim_seq_mon: monotone3 _sim_seq.
+  Proof.
+    unfold _sim_seq. ii. des. esplits; eauto.
+    { i. exploit NASTEP; eauto. i. des. esplits; eauto. }
+    { i. exploit ATSTEP; eauto. i. des. esplits; eauto.
+      i. exploit SIM; eauto. i. des. esplits; eauto. }
+  Qed.
+
+  Definition sim_seq := paco3 _sim_seq.
+End SIMULATION.
+#[export] Hint Resolve sim_seq_mon: paco.
+
+
+
 
 
 Module Oracle.
@@ -316,86 +348,10 @@ Module Oracle.
   Lemma step_wf e d o0 o1
         (STEP: step e d o0 o1)
     :
-      wf_diff d e.
+      wf_diff_event d e.
   Admitted.
 End Oracle.
 
-
-
-
-
-Module SeqState.
-Section LANG.
-  Variable lang: language.
-
-  Record t :=
-    mk {
-        state: lang.(Language.state);
-        memory: SeqMemory.t;
-      }.
-
-  (* without oracle *)
-  Variant na_local_step (p: Perms):
-    forall (e: MachineEvent.t)
-           (pe: ProgramEvent.t)
-           (m0: SeqMemory.t)
-           (m1: SeqMemory.t), Prop :=
-  | na_local_step_silent
-      m
-    :
-      na_local_step
-        p
-        (MachineEvent.silent) (ProgramEvent.silent)
-        m m
-  | na_local_step_read
-      m
-      loc val ord
-      (ORD: Ordering.le ord Ordering.na)
-      (VAL: Perm.le Perm.full (p loc) -> fst (m loc) = val)
-    :
-      na_local_step
-        p
-        (MachineEvent.silent) (ProgramEvent.read loc val ord)
-        m m
-  | na_local_step_write
-      m0 m1 e
-      loc val ord
-      (ORD: Ordering.le ord Ordering.na)
-      (MEM: SeqMemory.update loc val m0 = m1)
-      (PERM: e = if Perm.le Perm.full (p loc) then MachineEvent.silent else MachineEvent.failure)
-    :
-      na_local_step
-        p
-        e (ProgramEvent.write loc val ord)
-        m0 m1
-  | na_local_step_failure
-      m
-    :
-      na_local_step
-        p
-        (MachineEvent.failure) (ProgramEvent.failure)
-        m m
-  | na_local_step_update
-      m
-      loc valr valw ordr ordw
-      (ORD: __guard__(Ordering.le ordr Ordering.na \/ Ordering.le ordw Ordering.na))
-    :
-      na_local_step
-        p
-        (MachineEvent.failure) (ProgramEvent.update loc valr valw ordr ordw)
-        m m
-  .
-
-  Variant na_step (p: Perms): MachineEvent.t -> t -> t -> Prop :=
-  | na_step_intro
-      st0 st1 m0 m1 e pe
-      (LANG: lang.(Language.step) pe st0 st1)
-      (LOCAL: na_local_step p e pe m0 m1)
-    :
-      na_step p e (mk st0 m0) (mk st1 m1)
-  .
-End LANG.
-End SeqState.
 
 Module SeqThread.
 Section LANG.
@@ -426,247 +382,19 @@ Section LANG.
     - refl.
     - econs; eauto. econs; eauto.
   Qed.
-
-  Variant at_local_step (p: Perms):
-    forall (e: MachineEvent.t)
-           (pe: ProgramEvent.t)
-           (m0: SeqMemory.t)
-           (m1: SeqMemory.t), Prop :=
-  | na_local_step_silent
-      m
-    :
-      na_local_step
-        p
-        (MachineEvent.silent) (ProgramEvent.silent)
-        m m
-  | na_local_step_read
-      m
-      loc val ord
-      (ORD: Ordering.le ord Ordering.na)
-      (VAL: Perm.le Perm.full (p loc) -> fst (m loc) = val)
-    :
-      na_local_step
-        p
-        (MachineEvent.silent) (ProgramEvent.read loc val ord)
-        m m
-  | na_local_step_write
-      m0 m1 e
-      loc val ord
-      (ORD: Ordering.le ord Ordering.na)
-      (MEM: SeqMemory.update loc val m0 = m1)
-      (PERM: e = if Perm.le Perm.full (p loc) then MachineEvent.silent else MachineEvent.failure)
-    :
-      na_local_step
-        p
-        e (ProgramEvent.write loc val ord)
-        m0 m1
-  | na_local_step_failure
-      m
-    :
-      na_local_step
-        p
-        (MachineEvent.failure) (ProgramEvent.failure)
-        m m
-  | na_local_step_update
-      m
-      loc valr valw ordr ordw
-      (ORD: __guard__(Ordering.le ordr Ordering.na \/ Ordering.le ordw Ordering.na))
-    :
-      na_local_step
-        p
-        (MachineEvent.failure) (ProgramEvent.update loc valr valw ordr ordw)
-        m m
-  .
-
-  Variant at_step: MachineEvent.t -> t -> t -> Prop :=
-  | at_step_read
-      st0 st1
-      m0 p0 o0
-      loc val ord
-      m1 p1 o1
-      (STEP: lang.(Language.step) (ProgramEvent.read loc val ord) st0 st1)
-    :
-      at_step MachineEvent.silent (mk st0 m0 p0 o0) (mk st1 m1 p1 o1)
-  | at_step_write
-      st0 st1
-      m0 p0 o0
-      loc val ord
-      m1 p1 o1
-      (STEP: lang.(Language.step) (ProgramEvent.write loc val ord) st0 st1)
-    :
-      at_step MachineEvent.silent (mk st0 m0 p0 o0) (mk st1 m1 p1 o1)
-  | at_step_update
-      st0 st1
-      m0 p0 o0
-      loc valr valw ordr ordw
-      m1 p1 o1
-      (STEP: lang.(Language.step) (ProgramEvent.update loc valr valw ordr ordw) st0 st1)
-    :
-      at_step MachineEvent.silent (mk st0 m0 p0 o0) (mk st1 m1 p1 o1)
-  | at_step_fence
-      st0 st1
-      m0 p0 o0
-      ordr ordw
-      m1 p1 o1
-      (STEP: lang.(Language.step) (ProgramEvent.fence ordr ordw) st0 st1)
-    :
-      at_step MachineEvent.silent (mk st0 m0 p0 o0) (mk st1 m1 p1 o1)
-  | at_step_syscall
-      st0 st1
-      m0 p0 o0
-      e
-      m1 p1 o1
-      (STEP: lang.(Language.step) (ProgramEvent.syscall e) st0 st1)
-    :
-      at_step (MachineEvent.syscall e) (mk st0 m0 p0 o0) (mk st1 m1 p1 o1)
-  .
 End LANG.
-End State.
+End SeqThread.
 
-Section SIMULATION.
-  Variable lang_src: language.
-  Variable lang_tgt: language.
+Require Import ITreeLang.
+Require Import iCompatibility.
 
-  Variable sim_terminal: forall (st_src:(Language.state lang_src)) (st_tgt:(Language.state lang_tgt)), Prop.
+(* Section ADEQUACY. *)
+(*   Variable sim_terminal: *)
+(*     forall R_src R_tgt *)
+(*            (sim_ret:SIM_VAL R_src R_tgt) *)
+(*            (st_src: itree MemE.t R_src) (st_tgt: itree MemE.t R_tgt), Prop. *)
 
-  Definition SIM_SEQ :=
-    forall
-      (p: Perms)
-      (st_src: lang_src.(Language.state))
-      (mem_src: SeqMemory.t)
-      (st_tgt: lang_tgt.(Language.state))
-      (mem_tgt: SeqMemory.t), Prop.
+(*   Variable R_src R_tgt: Type. *)
 
-  Inductive _sim_seq
-            (sim_seq: SIM_SEQ)
-            (p: Perms)
-            (st_src0: lang_src.(Language.state))
-            (mem_src0: SeqMemory.t)
-            (st_tgt0: lang_tgt.(Language.state))
-            (mem_tgt0: SeqMemory.t): Prop :=
-  | sim_seq_step
-      (NASTEP: forall st_tgt1 e
-                      (STEP_TGT: State.na_step
-
-
-
-
-
-      (TERMINAL: forall (TERMINAL_TGT: (Language.is_terminal lang_tgt) st1_tgt),
-          (<<FAILURE: Thread.steps_failure (Thread.mk _ st1_src lc1_src sc1_src mem1_src)>>) \/
-          exists st2_src lc2_src sc2_src mem2_src w2,
-            (<<STEPS: rtc (@Thread.tau_step _)
-                          (Thread.mk _ st1_src lc1_src sc1_src mem1_src)
-                          (Thread.mk _ st2_src lc2_src sc2_src mem2_src)>>) /\
-            (<<SC: sim_timemap w2 sc2_src sc1_tgt>>) /\
-            (<<MEMORY: sim_memory w2 mem2_src mem1_tgt>>) /\
-            (<<TERMINAL_SRC: (Language.is_terminal lang_src) st2_src>>) /\
-            (<<LOCAL: sim_local w2 lc2_src lc1_tgt>>) /\
-            (<<TERMINAL: sim_terminal st2_src st1_tgt>>) /\
-            (<<WORLD: world_le w1 w2>>)>>) /\
-
-
-    (M<
-
-
-
-             (st1_src:(Language.state lang_src)) (lc1_src:Local.t) (sc0_src:TimeMap.t) (mem0_src:Memory.t)
-             (st1_tgt:(Language.state lang_tgt)) (lc1_tgt:Local.t) (sc0_tgt:TimeMap.t) (mem0_tgt:Memory.t): Prop :=
-    forall w1 sc1_src mem1_src
-           sc1_tgt mem1_tgt
-           (SC: sim_timemap w1 sc1_src sc1_tgt)
-           (MEMORY: sim_memory w1 mem1_src mem1_tgt)
-           (SC_FUTURE_SRC: TimeMap.le sc0_src sc1_src)
-           (SC_FUTURE_TGT: TimeMap.le sc0_tgt sc1_tgt)
-           (MEM_FUTURE_SRC: Memory.future_weak mem0_src mem1_src)
-           (MEM_FUTURE_TGT: Memory.future_weak mem0_tgt mem1_tgt)
-           (WF_SRC: Local.wf lc1_src mem1_src)
-           (WF_TGT: Local.wf lc1_tgt mem1_tgt)
-           (SC_SRC: Memory.closed_timemap sc1_src mem1_src)
-           (SC_TGT: Memory.closed_timemap sc1_tgt mem1_tgt)
-           (MEM_SRC: Memory.closed mem1_src)
-           (MEM_TGT: Memory.closed mem1_tgt)
-           (CONS_TGT: Local.promise_consistent lc1_tgt)
-           (WORLD: world_le w0 w1),
-      (<<TERMINAL:
-         forall (TERMINAL_TGT: (Language.is_terminal lang_tgt) st1_tgt),
-           (<<FAILURE: Thread.steps_failure (Thread.mk _ st1_src lc1_src sc1_src mem1_src)>>) \/
-           exists st2_src lc2_src sc2_src mem2_src w2,
-             (<<STEPS: rtc (@Thread.tau_step _)
-                           (Thread.mk _ st1_src lc1_src sc1_src mem1_src)
-                           (Thread.mk _ st2_src lc2_src sc2_src mem2_src)>>) /\
-             (<<SC: sim_timemap w2 sc2_src sc1_tgt>>) /\
-             (<<MEMORY: sim_memory w2 mem2_src mem1_tgt>>) /\
-             (<<TERMINAL_SRC: (Language.is_terminal lang_src) st2_src>>) /\
-             (<<LOCAL: sim_local w2 lc2_src lc1_tgt>>) /\
-             (<<TERMINAL: sim_terminal st2_src st1_tgt>>) /\
-             (<<WORLD: world_le w1 w2>>)>>) /\
-      (<<PROMISES:
-         forall (PROMISES_TGT: (Local.promises lc1_tgt) = Memory.bot),
-           (<<FAILURE: Thread.steps_failure (Thread.mk _ st1_src lc1_src sc1_src mem1_src)>>) \/
-           exists st2_src lc2_src sc2_src mem2_src,
-             (<<STEPS: rtc (@Thread.tau_step _)
-                           (Thread.mk _ st1_src lc1_src sc1_src mem1_src)
-                           (Thread.mk _ st2_src lc2_src sc2_src mem2_src)>>) /\
-             (<<PROMISES_SRC: (Local.promises lc2_src) = Memory.bot>>)>>) /\
-      (<<STEP: _sim_thread_step _ _ (@sim_thread lang_src lang_tgt sim_terminal)
-                                w1
-                                st1_src lc1_src sc1_src mem1_src
-                                st1_tgt lc1_tgt sc1_tgt mem1_tgt>>).
-
-
-  Inductive _sim
-            (sim:
-               forall
-                 (st_src: lang.(Language.state))
-                 (mem_src: SeqMemory.t)
-                 (p_src: Perms)
-                 (st_tgt: lang.(Language.state))
-                 (mem_tgt: SeqMemory.t)
-                 (p_tgt: Perms), Prop):
-    forall
-      (st_src: lang.(Language.state))
-      (mem_src: SeqMemory.t)
-      (p_src: Perms)
-      (st_tgt: lang.(Language.state))
-      (mem_tgt: SeqMemory.t)
-      (p_tgt: Perms), Prop :=
-  | sim_final
-      st_src mem_src p_src st_tgt mem_tgt p_tgt
-      (TGT: lang.(Language.is_terminal) st_tgt)
-      (SRC: lang.(Language.is_terminal) st_src)
-
-sim_thread
-
-
-  Definition SIM_TERMINAL (lang_src lang_tgt:language) :=
-    forall (st_src:(Language.state lang_src)) (st_tgt:(Language.state lang_tgt)), Prop.
-
-  Definition SIM_THREAD :=
-    forall (lang_src lang_tgt:language) (sim_terminal: SIM_TERMINAL lang_src lang_tgt)
-           (w: world)
-           (st1_src:(Language.state lang_src)) (lc1_src:Local.t) (sc0_src:TimeMap.t) (mem0_src:Memory.t)
-           (st1_tgt:(Language.state lang_tgt)) (lc1_tgt:Local.t) (sc0_tgt:TimeMap.t) (mem0_tgt:Memory.t), Prop.
-
-
-
-
-Language.t
-
-
-          state: lang.(Language.state);
-        memory: SeqMemory.t;
-        perm: Perms;
-
-
-
-
-Module Memory.
-  Definition t := Loc.t -> Cell.t.
-
-
-Memory.t
-
-Variant mem_permission
-
-ProgramEvent.t
+(*   Definition sim_seq_itree (st_src: itree MemE.t R_src) (st_tgt: itree MemE.t R_tgt): Prop := *)
+(*     forall p m, sim_seq (sim_terminal _ _) *)
